Cleanup and readme for thesis

src/Language/STLC/Alpha/alpha_subs.v
@@ -6,18 +6,17 @@ Require Import Coq.Program.Equality.
 Require Import ssreflect.
 
 (* One subsitution is related to the other through the alpha context*)
-Inductive αCtxSub : list (string * string) -> list (string * term) -> list (string * term) -> Set :=
-  | alpha_ctx_nil R : αCtxSub R [] []
+Inductive alphaSubs : list (string * string) -> list (string * term) -> list (string * term) -> Set :=
+  | alpha_ctx_nil R : alphaSubs R [] []
   | alpha_ctx_cons R σ σ' x y t t' :
-  (* TODO: what about sigma and sigma'? no conditions?*)
-    αCtxSub R σ σ' ->
+    alphaSubs R σ σ' ->
     AlphaVar R x y ->
     Alpha R t t' ->
-    αCtxSub R ((x, t)::σ) ((y, t')::σ').
+    alphaSubs R ((x, t)::σ) ((y, t')::σ').
 
 
 Lemma αctx_sym σ σ' R :
-  αCtxSub R σ σ' -> αCtxSub (sym_alpha_ctx R) σ' σ.
+  alphaSubs R σ σ' -> alphaSubs (sym_alpha_ctx R) σ' σ.
 Proof.
   intros Hctx.
   induction Hctx.
@@ -26,19 +25,8 @@ Proof.
   - eapply alpha_sym; eauto. apply sym_alpha_ctx_is_sym.
 Qed.
 
-(* 
-(* Not used? *)
-Lemma alpha_ctx_found ren sigma sigma' x x' t t' :
-  αCtxSub ren sigma sigma' ->
-  AlphaVar ren x x' ->
-  lookup x sigma = Some t ->
-  lookup x' sigma' = Some t' ->
-  Alpha ren t t'.
-Proof.
-Admitted. *)
-
 Lemma alpha_ctx_right_ex {ren sigma sigma' x x' t }:
-  αCtxSub ren sigma sigma' ->
+  alphaSubs ren sigma sigma' ->
   AlphaVar ren x x' ->
   lookup x sigma = Some t ->
   {t' & prod (lookup x' sigma' = Some t') (Alpha ren t t')}.
@@ -53,13 +41,13 @@ Proof.
   - remember H0 as Hav_xx'; clear HeqHav_xx'.
     apply (alphavar_unique_not_left H2 a) in H0.
     simpl in H1. rewrite <- String.eqb_neq in H2. rewrite H2 in H1.
-    specialize (IHαCtxSub Hav_xx' H1) as [t'0 [Hlookup Ha_t]].
+    specialize (IHalphaSubs Hav_xx' H1) as [t'0 [Hlookup Ha_t]].
     exists t'0. split; auto.
     simpl. rewrite <- String.eqb_neq in H0. rewrite H0. auto.
 Qed.
 
 Lemma alpha_ctx_left_ex {ren sigma sigma' x x' t' }:
-  αCtxSub ren sigma sigma' ->
+  alphaSubs ren sigma sigma' ->
   AlphaVar ren x x' ->
   lookup x' sigma' = Some t' ->
   { t & prod (lookup x sigma = Some t) (Alpha ren t t')}.
@@ -75,7 +63,7 @@ Proof.
 Qed.
 
 Lemma alpha_ctx_left_nex {ren sigma sigma' x x'}:
-  αCtxSub ren sigma sigma' ->
+  alphaSubs ren sigma sigma' ->
   AlphaVar ren x x' ->
   lookup x' sigma' = None ->
   lookup x sigma = None.
@@ -91,7 +79,7 @@ Proof.
 Qed.
 
 Lemma alpha_ctx_right_nex {ren sigma sigma' x x'}:
-  αCtxSub ren sigma sigma' ->
+  alphaSubs ren sigma sigma' ->
   AlphaVar ren x x' ->
   lookup x sigma = None ->
   lookup x' sigma' = None.
@@ -107,19 +95,19 @@ Proof.
 Qed.
 
 Lemma alpha_ctx_ren_nil {sigma }:
-  αCtxSub [] sigma sigma.
+  alphaSubs [] sigma sigma.
 Proof.
   induction sigma.
   - apply alpha_ctx_nil.
   - destruct a.
     apply alpha_ctx_cons; auto.
     + apply alpha_var_refl.
-    + apply alpha_refl. apply alpha_refl_nil.
+    + apply alpha_refl. apply id_ctx_nil.
 Qed.
 
 Lemma αctx_trans R1 R2 R σ σ' σ'' :
   αCtxTrans R1 R2 R -> 
-  αCtxSub R1 σ σ' -> αCtxSub R2 σ' σ'' -> αCtxSub R σ σ''.
+  alphaSubs R1 σ σ' -> alphaSubs R2 σ' σ'' -> alphaSubs R σ σ''.
 Proof.
   intros.
   dependent induction σ.
@@ -134,12 +122,8 @@ Proof.
     + eapply alpha_trans; eauto.
 Qed.
 
-(* Lemma αctx_ids idCtx σ σ' :
-  IdCtx idCtx -> αCtxSub nil σ σ' -> αCtxSub idCtx σ σ'.
-Admitted. *)
-
 Lemma αctx_sub_extend_ids_right σ σ' R1 R2 :
-  IdCtx R2 -> αCtxSub R1 σ σ' -> αCtxSub (R1 ++ R2) σ σ'.
+  IdCtx R2 -> alphaSubs R1 σ σ' -> alphaSubs (R1 ++ R2) σ σ'.
 Proof.
   intros HidR2 Ha.
   dependent induction σ.
