src/Util/List.v
@@ -739,3 +739,91 @@ Proof with auto using NameIn.
       apply NI_There...
       apply IHxs...
 Qed.
+
+
+(***** Set/prop trick for In ******)
+Inductive InSet {A : Type} (x : A) : list A -> Type :=
+| InSet_head : forall l, InSet x (x :: l)
+| InSet_tail : forall y l, InSet x l -> InSet x (y :: l).
+
+Lemma in_app_or_set {A} (x : A) (l1 l2 : list A) :
+  InSet x (l1 ++ l2) -> sum (InSet x l1) (InSet x l2).
+Proof.
+    induction l1 as [|h t IH]; simpl; intros H.
+  - right; exact H.
+  - inversion H; subst; clear H.
+    + left; apply InSet_head.
+    + destruct (IH X) as [H'|H'].
+      * left; apply InSet_tail; exact H'.
+      * right; exact H'.
+Qed.
+
+Definition in_dec_set {A} (eq_dec : forall x y : A, {x = y} + {x <> y}) (x : A) (l : list A) :
+  sum (InSet x l) ((InSet x l) -> False).
+Proof.
+  induction l as [|h t IH].
+  - right; intros H; inversion H.
+  - destruct (eq_dec x h) as [-> | Hneq].
+    + left; apply InSet_head.
+    + destruct IH as [Hin | Hnin].
+      * left; apply InSet_tail; exact Hin.
+      * right; intros H; inversion H; subst; [contradiction | apply Hnin; assumption].
+Defined.
+
+Theorem in_set_to_prop {A} {x : A} {l : list A} :
+  InSet x l -> In x l.
+Proof.
+  intros.
+  induction l as [|h t IH]; simpl in *.
+  - inversion X.
+  - inversion X; subst.
+    + left; reflexivity.
+    + right; apply IH; assumption.
+Qed.
+
+Fixpoint in_dec_f {A} (eq_dec : forall x y : A, {x = y} + {x <> y}) (x : A) (l : list A) :
+  bool:=
+  match l with
+  | [] => false
+  | h :: hs =>
+      match eq_dec x h with
+      | left _ => true
+      | right _ => in_dec_f eq_dec x hs
+      end
+  end.
+
+Theorem in_dec_f_sound {A} {eq_dec : forall x y : A, {x = y} + {x <> y}} {x : A} {l : list A} :
+  in_dec_f eq_dec x l = true -> InSet x l.
+Proof.
+  induction l as [|h t IH]; simpl; intros H.
+  - discriminate H.
+  - destruct (eq_dec x h) as [-> | Hneq].
+    + apply InSet_head.
+    + apply InSet_tail.
+      apply IH.
+      auto.
+Qed.
+
+Theorem in_prop_to_set {x : string} {l : list string} :
+  In x l -> InSet x l.
+Proof.
+  intros.
+  destruct (in_dec_f string_dec x l) eqn:BU.
+  - eapply in_dec_f_sound; eauto.
+  - exfalso.
+    induction l.
+    + inversion H.
+    + inversion H; subst.
+      simpl in BU.
+      destruct (string_dec x x).
+      * discriminate BU.
+      * contradiction.
+      * assert (in_dec_f string_dec x l = false).
+        {
+          simpl in BU.
+          destruct (string_dec x a).
+          - discriminate BU.
+          - auto.
+        }
+        eapply IHl; auto.
+Qed.
