src/Examples/TypeCheckTest.v
@@ -1,0 +1,16 @@
+From PlutusCert Require Import
+  PlutusIR
+  Typechecker
+.
+
+Require Import Coq.Strings.String.
+Open Scope string_scope.
+
+Require Import Lists.List.
+Import ListNotations.
+
+Definition t := (LamAbs "x" (Ty_Lam "α" Kind_Base (Ty_Var "α")) (Var "x")).
+
+Definition t_type := type_check [] [] t.
+
+
