src/Language/STLC/Alpha/alpha_kinding.v
@@ -1,7 +1,7 @@
 Require Import Coq.Lists.List.
 Require Import Coq.Strings.String.
 Import ListNotations.
-From PlutusCert Require Import variables util Alpha.alpha STLC KindingSTLC Util.List alpha_freshness alpha_rename.
+From PlutusCert Require Import variables util Alpha.alpha STLC STLC.Kinding Util.List alpha_freshness alpha_rename.
 Local Open Scope string_scope.
 Local Open Scope list_scope.
 
@@ -20,8 +20,8 @@ Inductive CAlpha : list (string * string) -> list (string * PlutusIR.kind) -> li
 Set Printing Implicit.
 
 (* Exercise and possibly useful *)
-Lemma alpha_preserves_typing sigma s t A Gamma Gamma' :
-  Alpha sigma s t -> CAlpha sigma Gamma Gamma' -> KindingSTLC.has_kind Gamma s A -> KindingSTLC.has_kind Gamma' t A.
+Lemma alpha_preserves_kinding sigma s t A Gamma Gamma' :
+  Alpha sigma s t -> CAlpha sigma Gamma Gamma' -> STLC.Kinding.has_kind Gamma s A -> STLC.Kinding.has_kind Gamma' t A.
 Proof.
   intros HAlpha Htype.
   generalize dependent A.
@@ -72,45 +72,4 @@ Proof.
   - intros.
     inversion H; subst.
     constructor. auto.
-Qed.
-
-Lemma substituteTCA_vacuous : forall R X U T T',
-    Alpha R T T' ->
-    ~ In X (ftv T) ->
-    Alpha R (substituteTCA X U T) T'.
-Proof.
-  intros.
-  generalize dependent T.
-  generalize dependent R.
-  induction T'; intros.
-  all: inversion H; subst.
-  all: autorewrite with substituteTCA.
-  - apply not_in_ftv_var in H0.
-    rewrite <- String.eqb_neq in H0.
-    now rewrite H0.
-  - destr_eqb_eq X x; [now constructor|].
-    assert (~ In X (ftv s1)) by now apply ftv_lam_negative in H0.
-    destruct (existsb (eqb x) (ftv U)) eqn:sinU.
-    + simpl.
-      remember (fresh2 _ s1) as Y.
-      constructor.
-      eapply IHT'.
-      * eapply alpha_trans_rename_left; eauto.
-      * apply ftv_not_in_rename; auto.
-        eapply fresh2_over_key_sigma in HeqY. symmetry. eauto.
-        apply in_eq.
-    + constructor; auto.
-  - constructor.
-    + eapply IHT'1; eauto. 
-      now apply not_ftv_app_not_left in H0.
-    + eapply IHT'2; eauto.
-      now apply not_ftv_app_not_right in H0.
-  - auto.
-Qed.
-
-Corollary substituteTCA_vacuous_specialized X U T:  
-  ~ In X (ftv T) ->
-  Alpha nil (substituteTCA X U T) T.
-Proof.
-  eapply substituteTCA_vacuous; try apply alpha_ids; auto; repeat constructor.
 Qed.
