src/Language/STLC/Scoping/GU_NC.v
@@ -10,7 +10,14 @@ Require Import Lia.
 Require Import Coq.Program.Basics.
 Require Import Coq.Arith.Arith.
 
-From PlutusCert Require Import STLC step_naive util Alpha.alpha variables alpha_freshness alpha_ctx_sub.
+From PlutusCert Require Import 
+STLC 
+step_naive 
+util 
+Alpha.alpha 
+variables 
+alpha_freshness 
+alpha_subs.
 
 
 
@@ -19,9 +26,8 @@ Hint Constructors Alpha : α_eq_db.
 Hint Resolve alpha_refl : α_eq_db.
 Hint Resolve alpha_sym : α_eq_db.
 Hint Resolve alpha_trans : α_eq_db.
-Hint Constructors AlphaCtxRefl : α_eq_db.
 Hint Constructors AlphaVar : α_eq_db.
-Hint Constructors αCtxSub : α_eq_db.
+Hint Constructors alphaSubs : α_eq_db.
 Hint Constructors AlphaCtxSym : α_eq_db.
 Hint Constructors αCtxTrans : α_eq_db.
 Hint Resolve alpha_extend_ids : α_eq_db.
